backend/Mach.v
@@ -270,7 +270,8 @@ Inductive state: Type :=
       forall (stack: list stackframe)  (**r call stack *)
              (f: block)                (**r pointer to function to call *)
              (rs: regset)              (**r register state *)
-             (m: mem),                 (**r memory state *)
+             (m: mem)                  (**r memory state *)
+             (id: ident),
       state
   | Returnstate:
       forall (stack: list stackframe)  (**r call stack *)
@@ -288,6 +289,12 @@ Definition parent_ra (s: list stackframe) : val :=
   match s with
   | nil => Vnullptr
   | Stackframe f sp ra c :: s' => ra
+  end.
+
+Definition ros_is_ident (ros: mreg + ident) (rs: regset) (i: ident) : Prop :=
+  match ros with
+  | inl r => rs r = Vptr (Global i) Ptrofs.zero
+  | inr symb => i = symb
   end.
 
 Inductive step: state -> trace -> state -> Prop :=
@@ -335,22 +342,25 @@ Inductive step: state -> trace -> state -> Prop :=
       step (State s f sp (Mstore chunk addr args src :: c) rs m)
         E0 (State s f sp c rs' m')
   | exec_Mcall:
-      forall s fb sp sig ros c rs m f f' ra,
+      forall s fb sp sig ros c rs m f f' ra id,
+      ros_is_ident ros rs id ->
       find_function_ptr ge ros rs = Some f' ->
       Genv.find_funct_ptr ge fb = Some (Internal f) ->
       return_address_offset f c ra ->
       step (State s fb sp (Mcall sig ros :: c) rs m)
         E0 (Callstate (Stackframe fb sp (Vptr fb ra) c :: s)
-                       f' rs m)
+                       f' rs m id)
   | exec_Mtailcall:
-      forall s fb stk soff sig ros c rs m f f' m',
+      forall s fb stk soff sig ros c rs m f f' m' m'' id,
+      ros_is_ident ros rs id ->
       find_function_ptr ge ros rs = Some f' ->
       Genv.find_funct_ptr ge fb = Some (Internal f) ->
       load_stack m (Vptr stk soff) Tptr f.(fn_link_ofs) = Some (parent_sp s) ->
       load_stack m (Vptr stk soff) Tptr f.(fn_retaddr_ofs) = Some (parent_ra s) ->
       Mem.free m stk 0 f.(fn_stacksize) = Some m' ->
+      Mem.return_frame m' = Some m'' ->
       step (State s fb (Vptr stk soff) (Mtailcall sig ros :: c) rs m)
-        E0 (Callstate s f' rs m')
+        E0 (Callstate s f' rs m'' id)
   | exec_Mbuiltin:
       forall s f sp rs m ef args res b vargs t vres rs' m',
       eval_builtin_args ge rs sp m args vargs ->
@@ -388,30 +398,32 @@ Inductive step: state -> trace -> state -> Prop :=
       step (State s fb sp (Mjumptable arg tbl :: c) rs m)
         E0 (State s fb sp c' rs' m)
   | exec_Mreturn:
-      forall s fb stk soff c rs m f m',
+      forall s fb stk soff c rs m f m' m'',
       Genv.find_funct_ptr ge fb = Some (Internal f) ->
       load_stack m (Vptr stk soff) Tptr f.(fn_link_ofs) = Some (parent_sp s) ->
       load_stack m (Vptr stk soff) Tptr f.(fn_retaddr_ofs) = Some (parent_ra s) ->
       Mem.free m stk 0 f.(fn_stacksize) = Some m' ->
+      Mem.return_frame m' = Some m'' ->
       step (State s fb (Vptr stk soff) (Mreturn :: c) rs m)
-        E0 (Returnstate s rs m')
+        E0 (Returnstate s rs m'')
   | exec_function_internal:
-      forall s fb rs m f m1 m2 m3 stk rs',
+      forall s fb rs m f m0 m1 m2 m3 stk rs' id path,
       Genv.find_funct_ptr ge fb = Some (Internal f) ->
-      Mem.alloc m 0 f.(fn_stacksize) = (m1, stk) ->
+      Mem.alloc_frame m id = (m0,path) ->
+      Mem.alloc m0 0 f.(fn_stacksize) = (m1, stk) ->
       let sp := Vptr stk Ptrofs.zero in
       store_stack m1 sp Tptr f.(fn_link_ofs) (parent_sp s) = Some m2 ->
       store_stack m2 sp Tptr f.(fn_retaddr_ofs) (parent_ra s) = Some m3 ->
       rs' = undef_regs destroyed_at_function_entry rs ->
-      step (Callstate s fb rs m)
+      step (Callstate s fb rs m id)
         E0 (State s fb sp f.(fn_code) rs' m3)
   | exec_function_external:
-      forall s fb rs m t rs' ef args res m',
+      forall s fb rs m t rs' ef args res m' id,
       Genv.find_funct_ptr ge fb = Some (External ef) ->
       extcall_arguments rs m (parent_sp s) (ef_sig ef) args ->
       external_call ef ge args m t res m' ->
       rs' = set_pair (loc_result (ef_sig ef)) res (undef_caller_save_regs rs) ->
-      step (Callstate s fb rs m)
+      step (Callstate s fb rs m id)
          t (Returnstate s rs' m')
   | exec_return:
       forall s f sp ra c rs m,
@@ -425,7 +437,7 @@ Inductive initial_state (p: program): state -> Prop :=
       let ge := Genv.globalenv p in
       Genv.init_mem p = Some m0 ->
       Genv.find_symbol ge p.(prog_main) = Some fb ->
-      initial_state p (Callstate nil fb (Regmap.init Vundef) m0).
+      initial_state p (Callstate nil fb (Regmap.init Vundef) m0 p.(prog_main)).
 
 Inductive final_state: state -> int -> Prop :=
   | final_state_intro: forall rs m r retcode,
@@ -443,9 +455,9 @@ Definition semantics (rao: function -> code -> ptrofs -> Prop) (p: program) :=
 Definition is_leaf_function (f: function) : bool :=
   List.forallb
     (fun i => match i with Mcall _ _ => false | _ => true end)
-    f.(fn_code).  
+    f.(fn_code).
 
-(** Semantic characterization of leaf functions: 
+(** Semantic characterization of leaf functions:
     functions in the call stack are never leaf functions. *)
 
 Section WF_STATES.
@@ -467,9 +479,9 @@ Inductive wf_state: state -> Prop :=
         (CODE: Genv.find_funct_ptr ge fb = Some (Internal f))
         (TAIL: is_tail c f.(fn_code)),
       wf_state (State s fb sp c rs m)
-  | wf_call_state: forall s fb rs m
+  | wf_call_state: forall s fb rs m id
         (STACK: Forall wf_frame s),
-      wf_state (Callstate s fb rs m)
+      wf_state (Callstate s fb rs m id)
   | wf_return_state: forall s rs m
         (STACK: Forall wf_frame s),
       wf_state (Returnstate s rs m).
@@ -483,14 +495,14 @@ Proof.
   constructor.
   constructor; auto. econstructor; eauto with coqlib.
   destruct (is_leaf_function f) eqn:E; auto.
-  unfold is_leaf_function in E; rewrite forallb_forall in E. 
+  unfold is_leaf_function in E; rewrite forallb_forall in E.
   symmetry. apply (E (Mcall sig ros)). eapply is_tail_in; eauto.
 - (* goto *)
-  assert (f0 = f) by congruence. subst f0. econstructor; eauto using find_label_tail.  
+  assert (f0 = f) by congruence. subst f0. econstructor; eauto using find_label_tail.
 - (* cond *)
-  assert (f0 = f) by congruence. subst f0. econstructor; eauto using find_label_tail.  
+  assert (f0 = f) by congruence. subst f0. econstructor; eauto using find_label_tail.
 - (* jumptable *)
-  assert (f0 = f) by congruence. subst f0. econstructor; eauto using find_label_tail.  
+  assert (f0 = f) by congruence. subst f0. econstructor; eauto using find_label_tail.
 - (* return *)
   inv STACK. inv H1. econstructor; eauto.
 Qed.
