backend/Tunnelingproof.v
@@ -363,12 +363,12 @@ Inductive match_states: state -> state -> Prop :=
       match_states (Block s f sp (Lcond cond args pc1 pc2 :: bb) ls m)
                    (State ts (tunnel_function f) sp (branch_target f pc1) tls tm)
   | match_states_call:
-      forall s f ls m ts tls tm
+      forall s f ls m ts tls tm id
         (STK: list_forall2 match_stackframes s ts)
         (LS: locmap_lessdef ls tls)
         (MEM: Mem.extends m tm),
-      match_states (Callstate s f ls m)
-                   (Callstate ts (tunnel_fundef f) tls tm)
+      match_states (Callstate s f ls m id)
+                   (Callstate ts (tunnel_fundef f) tls tm id)
   | match_states_return:
       forall s ls m ts tls tm
         (STK: list_forall2 match_stackframes s ts)
@@ -516,7 +516,7 @@ Definition measure (st: state) : nat :=
   | Block s f sp (Lbranch pc :: _) ls m => (count_gotos f pc * 2 + 1)%nat
   | Block s f sp (Lcond _ _ pc1 pc2 :: _) ls m => (Nat.max (count_gotos f pc1) (count_gotos f pc2) * 2 + 1)%nat
   | Block s f sp bb ls m => 0%nat
-  | Callstate s f ls m => 0%nat
+  | Callstate s f ls m id => 0%nat
   | Returnstate s ls m => 0%nat
   end.
 
@@ -598,15 +598,20 @@ Proof.
 - (* Lcall *)
   left; simpl; econstructor; split.
   eapply exec_Lcall with (fd := tunnel_fundef fd); eauto.
+  destruct ros; simpl in *. generalize (LS (R m0)).
+  intro. inv H1. eauto. congruence. auto.
   eapply find_function_translated; eauto.
   rewrite sig_preserved. auto.
   econstructor; eauto.
   constructor; auto.
   constructor; auto.
 - (* Ltailcall *)
-  exploit Mem.free_parallel_extends. eauto. eauto. intros (tm' & FREE & MEM'). 
+  exploit Mem.free_parallel_extends. eauto. eauto. intros (tm' & FREE & MEM').
+  exploit Mem.return_frame_parallel_extends; eauto. intros (tm'' & RET & MEM'').
   left; simpl; econstructor; split.
   eapply exec_Ltailcall with (fd := tunnel_fundef fd); eauto.
+  destruct ros; simpl in *. generalize (LS (R m0)).
+  intro. inv H. eauto. congruence. auto.
   eapply find_function_translated; eauto using return_regs_lessdef, match_parent_locset.
   apply sig_preserved.
   econstructor; eauto using return_regs_lessdef, match_parent_locset.
@@ -652,13 +657,15 @@ Proof.
   eauto. rewrite list_nth_z_map. change U.elt with node. rewrite H0. reflexivity. eauto.
   econstructor; eauto using locmap_undef_regs_lessdef.
 - (* Lreturn *)
-  exploit Mem.free_parallel_extends. eauto. eauto. intros (tm' & FREE & MEM'). 
+  exploit Mem.free_parallel_extends. eauto. eauto. intros (tm' & FREE & MEM').
+  exploit Mem.return_frame_parallel_extends; eauto. intros (tm'' & RET & MEM'').
   left; simpl; econstructor; split.
   eapply exec_Lreturn; eauto.
   constructor; eauto using return_regs_lessdef, match_parent_locset.
 - (* internal function *)
+  exploit Mem.alloc_frame_extends; eauto. intros (tm' & ALLOCF & MEM').
   exploit Mem.alloc_extends. eauto. eauto. apply Z.le_refl. apply Z.le_refl.
-  intros (tm' & ALLOC & MEM'). 
+  intros (tm'' & ALLOC & MEM'').
   left; simpl; econstructor; split.
   eapply exec_function_internal; eauto.
   simpl. econstructor; eauto using locmap_undef_regs_lessdef, call_regs_lessdef.
@@ -681,13 +688,14 @@ Lemma transf_initial_states:
   exists st2, initial_state tprog st2 /\ match_states st1 st2.
 Proof.
   intros. inversion H.
-  exists (Callstate nil (tunnel_fundef f) (Locmap.init Vundef) m0); split.
+  exists (Callstate nil (tunnel_fundef f) (Locmap.init Vundef) m0 (prog_main tprog)); split.
   econstructor; eauto.
   apply (Genv.init_mem_transf TRANSL); auto.
   rewrite (match_program_main TRANSL).
   rewrite symbols_preserved. eauto.
   apply function_ptr_translated; auto.
   rewrite <- H3. apply sig_preserved.
+  rewrite (match_program_main TRANSL).
   constructor. constructor. red; simpl; auto. apply Mem.extends_refl.
 Qed.
 
