common/Separation.v
@@ -917,3 +917,89 @@ Proof.
 - red; unfold j1; intros. destruct (eq_block b b1). congruence. rewrite D; auto.
 - red; unfold j1; intros. destruct (eq_block b0 b1). congruence. rewrite D in H9 by auto. congruence.
 Qed.
+
+Lemma alloc_frame_unchanged_on:
+  forall P m m' id path,
+    Mem.alloc_frame m id = (m',path) ->
+    Mem.unchanged_on P m m'.
+Proof.
+  intros.
+  constructor; simpl; eauto.
+  - intro. eapply Mem.support_alloc_frame_1 in H. apply H.
+  - intros. eapply Mem.perm_alloc_frame; eauto.
+  - intros. inv H. reflexivity.
+Qed.
+
+Lemma return_frame_unchanged_on:
+  forall P m m',
+    Mem.return_frame m = Some m' ->
+    Mem.unchanged_on P m m'.
+Proof.
+  intros.
+  constructor; simpl.
+  - apply Mem.sup_include_return_frame; eauto.
+  - intros. erewrite Mem.perm_return_frame; eauto. reflexivity.
+  - intros. unfold Mem.return_frame in H. destr_in H. inv H. reflexivity.
+Qed.
+
+Lemma alloc_frame_rule:
+  forall j m1 m2 P m1' m2' id path1 path2,
+    m2 |= minjection j m1 ** P ->
+    Mem.alloc_frame m1 id = (m1',path1) ->
+    Mem.alloc_frame m2 id = (m2',path2) ->
+    m2' |= minjection j m1' ** P.
+Proof.
+  intros j m1 m2 P m1' m2' id path1 path2 (INJ & RP & DISJ) H1 H2.
+  split;[|split].
+  - inv H1. inv H2. inv INJ. constructor; eauto.
+    inv mi_inj. constructor; eauto.
+    intros. apply mi_freeblocks. unfold Mem.valid_block in *; simpl in *.
+    eauto. intro. apply H. apply Mem.sup_incr_frame_in. auto.
+    intros.  unfold Mem.valid_block in *; simpl in *.
+    apply Mem.sup_incr_frame_in. eauto.
+  - eapply m_invar. eauto. eapply alloc_frame_unchanged_on; eauto.
+  - red; simpl; intros.
+    destruct H as (b0 & delta & JB & PERM).
+    eapply DISJ; eauto.
+    exists b0, delta; split; eauto.
+    rewrite Mem.perm_alloc_frame; eauto.
+Qed.
+
+Lemma alloc_frame_rule_2:
+  forall j m1 m2 P Q id m1' m2' path1 path2,
+    m2 |= mconj (minjection j m1) Q ** P ->
+    Mem.alloc_frame m1 id = (m1',path1) ->
+    Mem.alloc_frame m2 id = (m2',path2) ->
+    m2' |= mconj (minjection j m1') Q ** P.
+Proof.
+  intros j m1 m2 P Q id m1' m2' path1 path2 SEP H1 H2.
+  eapply frame_mconj. apply SEP.
+  apply mconj_proj1 in SEP.
+  eapply alloc_frame_rule in SEP; eauto.
+  eapply m_invar. apply mconj_proj2 in SEP. apply SEP.
+  eapply alloc_frame_unchanged_on; eauto.
+Qed.
+
+Lemma return_frame_parallel_rule:
+  forall m1 m1' m2 j P,
+    m2 |= minjection j m1 ** P ->
+    Mem.return_frame m1 = Some m1' ->
+    Mem.is_active (Mem.stack(Mem.support m2)) ->
+    exists m2', Mem.return_frame m2 = Some m2' /\
+    m2' |= minjection j m1' ** P.
+Proof.
+  intros m1 m1' m2  j P MINJ POP1 POP2.
+  exploit Mem.return_frame_parallel_inject. apply MINJ. eauto. eauto.
+  intros (m2' & POP & INJ). exists m2'.
+  destruct MINJ as (MINJ & PM & DISJ).
+  split. auto.
+  split; [|split].
+  - simpl in *. auto.
+  - eapply m_invar. eauto.
+    exploit return_frame_unchanged_on. eauto.
+    intros. apply H.
+  - red; intros. eapply DISJ. 2: eauto. simpl in H |- *.
+    decompose [ex and] H.
+    repeat eexists; eauto.
+    eapply Mem.perm_return_frame; eauto.
+Qed.
